DenotationalLean/Order/Functions.lean
@@ -83,4 +83,21 @@ theorem fixed_point [CPOB P] (f : Cont P P) : fixed f (fix_chain f) := by
     _ = ⨆ fc := by grind [insert_iter_bottom, Subtype.ext]
     _ = fix_chain f := by rfl
 
+theorem least_prefixed_point [CPOB P] (f : Cont P P) :
+  ∀ (p : P) , prefixed f p -> fix_chain f ⊑ p
+:= by
+  intro p h
+  have _ : ∀ (n : Nat) , f^[n] ⊥ ⊑ p := by
+    intro n
+    induction n with
+    | zero => grind [Nat.iterate, CPOB.is_bot]
+    | succ m h =>
+      rw [Function.iterate_succ']
+      have _ : f (f^[m] ⊥) ⊑ f p := by apply f.val.prop ; grind
+      have _ : f p ⊑ p := by grind [prefixed]
+      grind [PO.po_trans]
+  have _ : upper_bound (iter_bottom_chain f).set p :=
+    by grind [upper_bound, iter_bottom_chain]
+  have _ : lub_chain (iter_bottom_chain f) ⊑ p := by grind [lub_chain]
+  grind [fix_chain]
 end fix
